WIP: split counter -incr_left

split_counter.v
@@ -10,7 +10,7 @@ Definition create_counter :=
  Lam (Pair (Alloc (Nat 0)) (Alloc (Nat 0))).
 
 Definition atomic_increment :=
- Rec (LetIn (Load (Var 0)) (If (CAS (Var 1) (Var 0) (BinOp Add (Var 0) (Nat 1))) Unit (App (Var 2) (Var 1)))).
+ Rec (LetIn (Load (Var 1)) (If (CAS (Var 2) (Var 0) (BinOp Add (Var 0) (Nat 1))) Unit (App (Var 1) (Var 2)))).
 
 Definition incr_left :=
  Lam (App atomic_increment (Fst (Var 0))).
@@ -41,9 +41,14 @@ Proof. solve_inG. Qed.
 Section counter.
   Context `{SplitIG Σ, heapIG Σ, savedPredG Σ nat}.
 
-  Definition of_Readers (M : gmap nat (gname * nat)) :
+  Fixpoint of_Readers_rec (M : list (gname * nat)) i :
     gmap nat (excl (leibnizC (gname * nat))) :=
-    (λ r, Excl (r)) <$> M.
+    match M with
+    | [] => ∅
+    | r :: M' => <[i := Excl r]>(of_Readers_rec M' (S i))
+    end.
+
+  Definition of_Readers M := of_Readers_rec M 0.
 
   Definition ownReaders split_name M := own split_name (● (of_Readers M)).
 
@@ -51,17 +56,23 @@ Section counter.
 
   Definition counterN := nroot .@ "counter".
 
+  Definition except_counterN := ⊤ ∖ nclose counterN.
+  Lemma except_counterN_eq : except_counterN = ⊤ ∖ nclose counterN.
+  Proof. trivial. Qed.
+  Typeclasses Opaque except_counterN.
+  Opaque except_counterN.
+
   Definition reader_inv r v I :=
     (∃ ψ, saved_pred_own (fst r) ψ ∗
          if (decide (snd r < v)) then
-           I (snd r) ={⊤ ∖ nclose counterN}=∗ ψ (snd r) ∗ I (snd r)
+           ψ (snd r)
          else
-           ψ (snd r))%I.
+           I (snd r) ={except_counterN}=∗ ψ (snd r) ∗ I (snd r))%I.
 
   Definition CounterInv split_name l r I :=
     (∃ lv rv M, l ↦ (NatV lv) ∗ r ↦ (NatV rv) ∗ I (lv + rv)
                   ∗ ownReaders split_name M
-                  ∗ [∗ map] i ↦ r ∈ M, reader_inv r (lv + rv) I)%I.
+                  ∗ [∗ list] r ∈ M, reader_inv r (lv + rv) I)%I.
 
   Definition Counter split_name (c : val) (I : nat → iProp Σ) : iProp Σ:=
   (∃ l r, ⌜c = PairV (LocV l) (LocV r)⌝ ∗ inv counterN (CounterInv split_name l r I))%I.
@@ -80,13 +91,64 @@ Section counter.
     iMod (own_alloc (A := authUR (gmapUR nat (exclR (leibnizC (gname * nat))))) (● ∅))
       as (split_name) "He"; first done.
     iMod (inv_alloc counterN _ (CounterInv split_name l r I) with "[-HF]") as "HI".
-    { iExists _, _, ∅; rewrite /ownReaders /of_Readers fmap_empty big_sepM_empty;
-        iFrame. }
+    { iExists _, _, []; rewrite /ownReaders /=; iFrame. }
     iApply wp_value.
     iApply "HF". iExists _, _; eauto.
   Qed.
 
-
-
-
+  Theorem wp_incr_left split_name c I Q :
+    {{{Counter split_name c I ∗ ∀ v, I v ={except_counterN}=∗ I (v +1) ∗ Q}}}
+      App incr_left (of_val c)
+    {{{RET UnitV; Q}}}.
+  Proof.
+    iIntros (F) "[#HInv Hvs] HF". iDestruct "HInv" as (l r ->) "HInv".
+    iApply wp_pure_step_later; auto. iNext. asimpl.
+    iApply (wp_bind (fill [AppRCtx (RecV _)])); simpl.
+    iApply wp_pure_step_later; auto. iNext.
+    iApply wp_value; simpl.
+    iLöb as "IH".
+    iApply wp_pure_step_later; auto. iNext. asimpl.
+    iApply (wp_bind (fill [LetInCtx _])); simpl.
+    iInv counterN as (lv rv M) "(Hl & Hr & HI & HM & Hri)" "Hcl".
+    iApply (wp_load with "Hl"). iNext. iIntros "Hl".
+    iMod ("Hcl" with "[Hl Hr HI HM Hri]") as "_".
+    { iNext; iExists _, _, _; iFrame. }
+    iModIntro.
+    iApply wp_pure_step_later; auto. iNext.
+    iApply (wp_bind (fill [IfCtx _ _])); simpl.
+    iApply (wp_bind (fill [CasRCtx (LocV _) (NatV _)])); simpl.
+    iApply wp_pure_step_later; auto. iNext.
+    iApply wp_value; simpl.
+    clear rv M.
+    iInv counterN as (lv' rv M) "(Hl & Hr & HI & HM & Hri)" "Hcl".
+    destruct (decide (lv = lv')); first subst.
+    - iApply (wp_cas_suc with "Hl"); iNext; iIntros "Hl".
+      iAssert (I (lv' + rv) ={⊤ ∖ ↑counterN}=∗ I (lv' + rv) ∗
+               [∗ list] r ∈ M, reader_inv r ((lv' + 1) + rv) I)%I
+        with "[Hri]" as "Hri'".
+      { iIntros "HI".
+        iInduction M as [|x M] "IHM"; simpl; first by iFrame.
+        iDestruct "Hri" as "[Hx HM]". iDestruct "Hx" as (ψ) "[Hψ Hx]".
+        iMod ("IHM" with "HM HI") as "[HI $]".
+        rewrite /reader_inv /=.
+        repeat destruct decide; simpl; try (by iFrame; eauto with omega).
+        replace (x.2) with (lv' + rv) by omega.
+        rewrite !except_counterN_eq.
+        iMod ("Hx" with "HI") as "[Hx $]"; eauto. }
+      iMod ("Hri'" with "HI") as "[HI Hri]".
+      rewrite !except_counterN_eq.
+      iMod ("Hvs" with "HI") as "[HI HQ]".
+      iMod ("Hcl" with "[Hl Hr HI HM Hri]") as "_".
+      { replace (lv' + rv + 1) with (lv' + 1 + rv) by omega.
+        iNext; iExists _, _, _; iFrame. }
+      iModIntro.
+      iApply wp_pure_step_later; auto. iNext.
+      by iApply wp_value; iApply "HF".
+    - iApply (wp_cas_fail with "Hl"); first congruence; iNext; iIntros "Hl".
+      iMod ("Hcl" with "[Hl Hr HI HM Hri]") as "_".
+      { iNext; iExists _, _, _; iFrame. }
+      iModIntro.
+      iApply wp_pure_step_later; auto. iNext.
+      iApply ("IH" with "Hvs"); eauto.
+  Qed.
 
